## Part 2a

$\textrm{index} = \sum_{i=1}^{d} (x_i\prod_{j=1}^{d-i} L_j)$

$x_1 = \textrm{index}\%L_1$

$x_i = \textrm{floor}(\dfrac{\textrm{index}\%(\prod_{j=1}^{i} L_j)}{\prod_{j=1}^{i-1}L_j})$


### For example
L = (4,8,5,9,6,7)

index = 1\*(4\*8\*5\*9\*6) + 2\*(4\*8\*5\*9) + 3\*(4\*8\*5) 7\*(4\*8) + 5\*(4) + 4

(1,2,3,7,5,4) = 42985

x1 = 42985%4 = 1

x2 = int((42985%(4\*8))/4) = 2

x3 = int(42985%(4\*8\*5)/(4\*8)) = 3

x4 = int(42985%(4\*8\*5\*9)/(4\*8\*5)) = 7

x5 = int(42985%(4\*8\*5\*9\*6)/(4\*8\*5\*9)) = 5

x6 = int(42985%(4\*8\*5\*9\*6\*7)/(4\*8\*5\*9\*6)) = 4
